src/LensPerms.v
@@ -188,22 +188,27 @@ Section PLensPerms.
   the value contained at ix, then if you read from ix (resulting in a predicate
   pred that ensures the value at ix = elem) then you get back a read_dep or
   write_dep with a value equal to elem, to which you also have permissions P *)
-  Lemma ixplens_read_ent rw ix P elem (pred : St -> Prop) :
-    (forall x, pred x -> iget ix x = Some elem) ->
-    add_poss_pre pred (ixplens_dep rw ix P)
-      ⊨ ixplens_dep rw ix (fun e => prop_Perms (e = elem)) * P elem.
+  Lemma ixplens_read_ent rw ix P opt_elem (pred : St -> Prop) :
+    (forall x, pred x -> iget ix x = opt_elem) ->
+    add_poss_pre pred (ixplens_dep rw ix P) ⊨
+      meet_Perms
+      (fun R =>
+         exists elem,
+           opt_elem = Some elem /\
+             R = ixplens_dep rw ix (fun e => prop_Perms (e = elem)) * P elem).
   Proof.
-    intro. apply add_poss_pre_meet_ent. intros. destruct H0; subst.
+    intro. apply add_poss_pre_meet_ent. intros. destruct H0 as [elem ?]; subst.
+    apply ent_meet_Perms. eexists.
+    assert (opt_elem = Some elem).
+    1: { apply Perms_field_conj_elim in H1. destruct H1.
+         apply Perms_field_singleton_elim in H0.
+         destruct H0 as [[? [? ?]] ?]. subst. specialize (H x H2).
+         rewrite H0 in H. symmetry; assumption. }
+    split; [ exists elem; split; [ assumption | reflexivity ] | ].
     etransitivity; [ apply add_pre_ent_P | ].
     unfold ixplens_dep. rewrite sep_conj_Perms_meet_commute.
     eapply ent_meet_Perms.
     eexists; split; [ eexists; split; [ reflexivity | exists elem; reflexivity ] | ].
-    assert (x0 = elem).
-    1: { apply Perms_field_conj_elim in H1. destruct H1.
-         apply Perms_field_singleton_elim in H0. destruct H0.
-         unfold Perms_field in H1; simpl in H1.
-         destruct rw; simpl in H0; destruct_ex_conjs H0; subst; rewrite (H _ H2) in H0;
-         inversion H0; reflexivity. }
     erewrite (proj2 (prop_Perms_bottom _)); [ | reflexivity ]. subst.
     rewrite (sep_conj_Perms_commut _ bottom_Perms).
     rewrite sep_conj_Perms_bottom_identity.
