src/LensTypes.v
@@ -1,0 +1,50 @@
+
+From Coq Require Import
+         Lists.List.
+
+From ITree Require Import
+     ITree
+     ITreeFacts.
+
+From Heapster Require Import
+     Utils
+     Permissions
+     Lifetime
+     SepStep
+     Typing
+     PermType
+     LensPerms.
+
+Import ITreeNotations.
+Import ListNotations.
+Local Open Scope itree_scope.
+
+
+Section PLensTypes.
+  Context {Si Ss Ix Elem : Type} {IxPLens:IxPartialLens Ix Si Elem}.
+
+
+  (***
+   *** The permission type associated with an indexed partial lens
+   ***)
+
+  Definition ixplensTp {Bs} rw (T : @PermType Si Ss Elem Bs) : PermType Ix Bs :=
+    mkPermType (fun ix bs => ixplens_dep rw ix (fun elem => ptApp T elem bs)).
+
+  Lemma ixplensRead Bs Ri Rss T (U : PermType Ri Rss) rw ix (bs : tuple Bs) ti ts :
+    (forall elem,
+        (ix :: ixplensTp rw (eqTp elem) ▷ tt * elem :: T ▷ bs)
+          ⊢ ti elem ⤳ ts ::: U) ->
+    ix :: ixplensTp rw T ▷ bs ⊢ (elem <- readIx ix;; ti elem) ⤳ ts ::: U.
+  Proof.
+    intro.
+    rewrite <- (bind_ret_l tt (fun x => ts)).
+    eapply typing_bind; [ | intros; apply H ].
+    unfold readIx. rewrite <- (bind_ret_l tt (fun x => Ret tt)).
+    eapply typing_bind; [ apply typing_read_L | ]. intros. simpl.
+    rewrite (ixplens_read_ent _ _ _ (iget ix r1));
+      [ | intros; destruct x; subst; reflexivity ].
+    apply typing_meet. intros.
+    destruct H0 as [elem [? ?]]; subst.
+    rewrite H0. simpl. apply typing_ret. reflexivity.
+  Qed.
